parameterized_chainmail_coq/L_def.v
@@ -19,20 +19,108 @@ Module Type LanguageDef.
   Notation "'⟦' σ '⟧'" := (config_translation σ)(at level 40) : L_scope.
 
   (* read visibility *)
-  Parameter visible_r : config -> addr -> value -> Prop.
+  Parameter visible_r : mdl -> config -> addr -> value -> Prop.
   (* write visibility *)
-  Parameter visible_w : config -> addr -> addr -> fld -> Prop.
+  Parameter visible_w : mdl -> config -> addr -> addr -> fld -> Prop.
   (* method visibility *)
-  Parameter visible_m : config -> addr -> addr -> mth -> Prop.
+  Parameter visible_m : mdl -> config -> addr -> addr -> mth -> Prop.
   (* constructor visibility *)
-  Parameter visible_c : config -> addr -> cls -> Prop.
+  Parameter visible_c : mdl -> config -> addr -> cls -> Prop.
+
+  Parameter visible_r_stack_append :
+    forall M σ α v, visible_r M σ α v ->
+               forall ψ, visible_r M (σ ◁ ψ) α v.
+
+  Parameter visible_w_stack_append :
+    forall M σ α1 α2 f, visible_w M σ α1 α2 f ->
+                   forall ψ, visible_w M (σ ◁ ψ) α1 α2 f.
+
+  Parameter visible_m_stack_append :
+    forall M σ α1 α2 m, visible_m M σ α1 α2 m ->
+                   forall ψ, visible_m M (σ ◁ ψ) α1 α2 m.
+
+  Parameter visible_c_stack_append :
+    forall M σ α C, visible_c M σ α C ->
+               forall ψ, visible_c M (σ ◁ ψ) α C.
 
   (* access *)
   Parameter has_access : mdl -> mdl -> config -> addr -> addr -> Prop.
 
   Parameter access_implies_read_visibility :
     forall M1 M2 σ α1 α2, has_access M1 M2 σ α1 α2 ->
-                     visible_r σ α1 (v_addr α2).
+                     forall M, M1 ⋄ M2 ≜ M ->
+                     visible_r M σ α1 (v_addr α2).
+
+  Ltac visible_stack_append_auto :=
+    match goal with
+    | [H : visible_r ?M (?χ, ?ϕ :: nil) ?α ?v
+       |- visible_r ?M (?χ, ?ϕ :: ?ψ') ?α ?v] =>
+      apply visible_r_stack_append with (ψ:=ψ') in H;
+      auto
+    | [H : visible_w ?M (?χ, ?ϕ :: nil) ?α1 ?α2 ?f
+       |- visible_w ?M (?χ, ?ϕ :: ?ψ') ?α1 ?α2 ?f] =>
+      apply visible_w_stack_append with (ψ:=ψ') in H;
+      auto
+    | [H : visible_m ?M (?χ, ?ϕ :: nil) ?α1 ?α2 ?m
+       |- visible_m ?M (?χ, ?ϕ :: ?ψ') ?α1 ?α2 ?m] =>
+      apply visible_m_stack_append with (ψ:=ψ') in H;
+      auto
+    | [H : visible_c ?M (?χ, ?ϕ :: nil) ?α ?C
+       |- visible_c ?M (?χ, ?ϕ :: ?ψ') ?α ?C] =>
+      apply visible_c_stack_append with (ψ:=ψ') in H;
+      auto
+
+    | [H : visible_r ?M (?χ, ?ψ) ?α ?v
+       |- visible_r ?M (?χ, ?ψ ++ ?ψ') ?α ?v] =>
+      apply visible_r_stack_append with (ψ:=ψ') in H;
+      auto
+    | [H : visible_w ?M (?χ, ?ψ) ?α1 ?α2 ?f
+       |- visible_w ?M (?χ, ?ψ ++ ?ψ') ?α1 ?α2 ?f] =>
+      apply visible_w_stack_append with (ψ:=ψ') in H;
+      auto
+    | [H : visible_m ?M (?χ, ?ψ) ?α1 ?α2 ?m
+       |- visible_m ?M (?χ, ?ψ ++ ?ψ') ?α1 ?α2 ?m] =>
+      apply visible_m_stack_append with (ψ:=ψ') in H;
+      auto
+    | [H : visible_c ?M (?χ, ?ψ) ?α ?C
+       |- visible_c ?M (?χ, ?ψ ++ ?ψ') ?α ?C] =>
+      apply visible_c_stack_append with (ψ:=ψ') in H;
+      auto
+
+    | [H : visible_r ?M (?χ, ?ϕ :: ?ψ) ?α ?v
+       |- visible_r ?M (?χ, ?ϕ :: ?ψ ++ ?ψ') ?α ?v] =>
+      apply visible_r_stack_append with (ψ:=ψ') in H;
+      auto
+    | [H : visible_w ?M (?χ, ?ϕ :: ?ψ) ?α1 ?α2 ?f
+       |- visible_w ?M (?χ, ?ϕ :: ?ψ ++ ?ψ') ?α1 ?α2 ?f] =>
+      apply visible_w_stack_append with (ψ:=ψ') in H;
+      auto
+    | [H : visible_m ?M (?χ, ?ϕ :: ?ψ) ?α1 ?α2 ?m
+       |- visible_m ?M (?χ, ?ϕ :: ?ψ ++ ?ψ') ?α1 ?α2 ?m] =>
+      apply visible_m_stack_append with (ψ:=ψ') in H;
+      auto
+    | [H : visible_c ?M (?χ, ?ϕ :: ?ψ) ?α ?C
+       |- visible_c ?M (?χ, ?ϕ :: ?ψ ++ ?ψ') ?α ?C] =>
+      apply visible_c_stack_append with (ψ:=ψ') in H;
+      auto
+
+    | [H : visible_r ?M (?χ, ?ϕ1 :: ?ϕ2 :: ?ψ) ?α ?v
+       |- visible_r ?M (?χ, ?ϕ1 :: ?ϕ2 :: ?ψ ++ ?ψ') ?α ?v] =>
+      apply visible_r_stack_append with (ψ:=ψ') in H;
+      auto
+    | [H : visible_w ?M (?χ, ?ϕ1 :: ?ϕ2 :: ?ψ) ?α1 ?α2 ?f
+       |- visible_w ?M (?χ, ?ϕ1 :: ?ϕ2 :: ?ψ ++ ?ψ') ?α1 ?α2 ?f] =>
+      apply visible_w_stack_append with (ψ:=ψ') in H;
+      auto
+    | [H : visible_m ?M (?χ, ?ϕ1 :: ?ϕ2 :: ?ψ) ?α1 ?α2 ?m
+       |- visible_m ?M (?χ, ?ϕ1 :: ?ϕ2 :: ?ψ ++ ?ψ') ?α1 ?α2 ?m] =>
+      apply visible_m_stack_append with (ψ:=ψ') in H;
+      auto
+    | [H : visible_c ?M (?χ, ?ϕ1 :: ?ϕ2 :: ?ψ) ?α ?C
+       |- visible_c ?M (?χ, ?ϕ1 :: ?ϕ2 :: ?ψ ++ ?ψ') ?α ?C] =>
+      apply visible_c_stack_append with (ψ:=ψ') in H;
+      auto
+    end.
 
   (*operational semantics*)
   Parameter L_red : mdl -> mdl -> L_config -> L_config -> Prop.
